[reconfiguration] supporting adding validators
- Added the additions vector to the LibraSystem.ValidatorSet resource. This vector tracks the list of addresses to be added to the validator set at the time of the next epoch.
- Added LibraSystem.add_validator(addr) procedure that can only be invoked by the Association. This procedure will cause the validator whose ValidatorConfig is stored at addr to be added to the validator set at the next epoch change.
- Modified  LibraSysterm.reconfigure() to add each address in the additions vector to the validator set.
- E2E tests for addition flow, authentication of add_validator, error cases of add_validator, interaction with key rotation

language/vm/vm-genesis/src/lib.rs
@@ -292,7 +292,7 @@ pub fn encode_genesis_transaction_with_validator(
                     vec![],
                 )
                 .unwrap();
-            for validator_keys in validator_set.payload() {
+            for validator_keys in validator_set.payload().iter().rev() {
                 // First, add a ValidatorConfig resource under each account
                 let validator_address = *validator_keys.account_address();
                 txn_executor.create_account(validator_address).unwrap();
@@ -378,7 +378,6 @@ pub fn encode_genesis_transaction_with_validator(
                 "Expected sequence number 0 for validator set change event but got {}",
                 validator_set_change_event.sequence_number()
             );
-
             // (4) It should emit the validator set we fed into the genesis tx
             assert_eq!(
                 ValidatorSet::from_bytes(validator_set_change_event.event_data()).unwrap(),
